# **--HW2 for FoPL**

--Stu:**金泽文** No:PB15111604

--This time, i tried to finish the homework in English, 
--which was so interesting.

1.
(**with** renaming)

``(λp.λq.λr.p q r)(λp.λq.p q r)``

`->  (λx.λy.λz.x y z)(λp.λq.p q r)       (rename)`
`->  λy.λz.(λp.λq.p q r) y z             (x -> (λp.λq.p q r))`
`->  λy.λz.(λq.y q r) z                  (p -> y)` 
`->  λy.λz.y z r                         (q -> z)`

(**without** renaming)

`(λp.λq.λr.p q r)(λp.λq.p q r)`

`->  λq.λr.(λp.λq.p q r) q r`
`->  λq.λr.(λq.q q r) r`
`->  λq.λr.(λr.r r r)`
`->  λr.(λr.r r r)`
The free **r** on the right will be **bound** because of the left one which is bound.

-----------------------------------------------
2.
definition of f in the form of lambda calculus :
    f = λg.g g
reduce the f(f) :
        f f 
    ->  (λg.g g) (λg.g g)
    ->  (λg.g g) (λg.g g)
    ->  ...

-----------------------------------------------
3.
(a)If the evaluation is the **lazy** one, then e1 and e2 may be evaluated only if the value is needed. On this occasion, the g process has to **wait** **until** e1 is evaluated and the then evaluate e1 = 0, after which the g process may also have to be wait for the e2 to be evaluated.

(b)With the lazy evaluation, it will be **fine** **and won't terminate with an error**, for e1=0 is True and g(e1, e2) will then return 1 without evaluating the e1 + e2.(It's just so lazy!)

(c)First, the error message from the e2 process **shouldn't influence** the g process. So the g process **shouldn't accept or wait** for the result of the other process **unless** it needs it. With this mechanism, e1 and e2 will be evaluated but only the value of e1 will be waited and accepted by the g process, and the g process get the True and return 1, without wating for the message from the e2 process.

(d)**I can't.** First, I don't know so parrelism so well, so I don't know if the e2, which contains an assignment to z will definitely be calculated before e1 or after e2. So I suppose the order can't be predicated. So if we still evaluate the arguments of g(e1, e2) in parallel, it may cause bad side-effects.
**But!!**If there is some good mechanism which can predicate the order of e1 and e2, then I will do it in parallel!

-----------------------------------------------
4.
(a) 
Haskel:    the **frist** one in the list.
C:         the **last** one in the list.

(b)Of course the **Hakell** one! Fisrt, it's so **short**! When I first saw the five-line-wonderful-code, I was **shocked**! It conveys **all** the algorithm I need without any nonsense! Even if I were a fresh one, when I see it I'll soon know the meanings and understand the algorithm! It's just the way we write in mathematics! But what's wrong with the C code? It's too long!

(c)
```haskell
q [] = [] 
q (x:xs) = q xl ++ [x] ++ q xr 
    where   (xl,xr,_) = until f g ([],[],xs) 
            f (_,_,w) = w==[] 
            g (l,g,y:ys) | y <= x = (y:l,g,ys) 
                         | y > x = (l,y:g,ys) 
```

the code above will only be computed only one pass once.

(d)
replace: 

```c
p = a[hi];
```

with:

```c
srand((unsigned int)(time(NULL));
p = (rand() % (hi-lo+1))+lo;
t = a[p];
a[p] = a[hi];
a[hi] = t;
p = a[hi];
```
I just generate one random int p and swap a[p] with a[hi].
The rest are the same.

(e)I guess each time  

```haskell
elts_lt_x = [y | y <- xs, y < x]
```

is processed, the space of (length elts_lt_x) * SOME_NUMBER will be used, for Haskell won't change the old value of the variables, so it will only use new spaces for new variables.
On this occasion, there will be **much more spaces** to be used than the C one.

-----------------------------------------------
5.
(a)
    <x + y, σ>  
`→   <_2_ + _y_, σ>` 
`→   <_2_ + _3_, σ>` 
`→   <_5_ ,σ>` 

(b)
    <x = x + 3, σ>
        --σ(x) = 1
`→  <x = 1 + 3, σ>`      
        --<n + m, σ> → <p, σ>
        --<1 + 3, σ> → <4, σ>
`→   <x = 4, σ>`          
        --<x = n, σ> → <n,Put(σ, x, n)>
`→   <4, Put(σ,x,4)>`     

(c)
    <(x = 3) + x, σ> 
        --<x = n, σ> → <n,Put(σ, x, n)>
        --<x = 3, σ> → <3,Put(σ, x, 3)>
`→   <3 + x, Put(σ,x,3)>`     
        --Put(σ,x,3)(x) = 3
`→   <3 + 3, Put(σ,x,3)>`     
        --<n + m, Put(σ,x,3)> → <p, Put(σ,x,3)>
        --<3 + 3, Put(σ,x,3)> → <6, Put(σ,x,3)>
`→   <6, Put(σ,x,3)>`         

(d)
    <x = (x = x + 3) + (x = x + 5), σ>
        --σ(x) = 1
`→    <x = (x = 1 + 3) + (x = x + 5), σ>`  
        --<n + m, σ> → <p, σ>
        --<1 + 3, σ> → <4, σ>
`→    <x = (x = 4) + (x = x + 5), σ>`      
        --<x = n, σ> → <n,Put(σ, x, n)>
        --<x = 4, σ> → <4,Put(σ, x, 4)>
`→    <x = 4 + (x = x + 5), Put(σ, x, 4)>`      
        --Put(σ, x, n)(x) = 4
`→    <x = 4 + (x = 4 + 5), Put(σ, x, 4)>`   
        --<n + m, Put(σ,x,4)> → <p, Put(σ,x,4)>   
        --<4 + 5, Put(σ,x,4)> → <9, Put(σ,x,4)>   
`→    <x = 4 + (x = 9), Put(σ, x, 4)>`   
        --<x = n, σ> → <n,Put(σ, x, n)>
        --<x = n, Put(σ, x, 4)> → <n,Put(Put(σ, x, 4), x, n)>
        --<x = 9, Put(σ, x, 4)> → <9,Put(Put(σ, x, 4), x, 9)>
`→    <x = 4 + 9, Put(σ, x, 9)>` 
        --<n + m, Put(σ,x,9)> → <p, Put(σ,x,9)>   
        --<4 + 9, Put(σ,x,9)> → <13, Put(σ,x,9)>
`→    <x = 13, Put(σ, x, 9)>` 
        --<x = n, σ> → <n,Put(σ, x, n)>
        --<x = 13, Put(σ, x, 4)> → <13,Put(Put(σ, x, 4), x, 13)>
`→    <13, Put(σ, x, 13)>` 


